

MASSACHUSETTS INSTITUTE OF TECHNOLOGY
ENTRANCE EXAMINATION, 1869-70
ALGEBRA

1. If $e=8$ find the numerical value of the following expression:

$$e - \{\sqrt{e+1} + 2\} + (e - \sqrt[3]{e})\sqrt{e-4}$$

The solution becomes really easy when you notice that $8 = 2^3$,

$$8 - \{\sqrt{8+1} + 2\} + (8 - \sqrt[3]{2^3})\sqrt{8-4} =$$

$$= 8 - \{\sqrt{9} + 2\} + (8 - 2)\sqrt{4} =$$

$$= 8 - \{3 + 2\} + (6) \times 2 =$$

$$= 8 - 5 + 12 = 3 + 12 = 15$$

2. Simplify the following expression by removing the brackets and collecting like terms

$$3a - [b + (2a - b) - (a - b)]$$

Once again, the trick is working with no hurries,

$$3a - [b + (2a - b) - (a - b)] = 3a - [b + 2a - b - a + b] = 3a - [b + a] = 2a - b$$

3. Multiply $3a^2 + ab - b^2$ by $a^2 - 2ab - 3b^2$ and divide the product by $a + b$

Step 1: Multiply the polynomials

$$(3a^2 + ab - b^2)(a^2 - 2ab - 3b^2)$$

Distributing each term:

$$= 3a^2(a^2 - 2ab - 3b^2) + ab(a^2 - 2ab - 3b^2) - b^2(a^2 - 2ab - 3b^2)$$

$$= 3a^4 - 6a^3b - 9a^2b^2 + a^3b - 2a^2b^2 - 3ab^3 - a^2b^2 + 2ab^3 + 3b^4$$

$$= 3a^4 - 5a^3b - 12a^2b^2 - ab^3 + 3b^4$$

Step 2: Divide by $(a + b)$

We perform polynomial long division:

$$\begin{array}{r|l} a + b & 3a^4 - 5a^3b - 12a^2b^2 - ab^3 + 3b^4 \\ & 3a^3 - 8a^2b - 4ab^2 + 3b^3 \hline \end{array}$$

Therefore:

$$\boxed{3a^3 - 8a^2b - 4ab^2 + 3b^3}$$

Appendix: Detailed Long Division Process

We divide $3a^4 - 5a^3b - 12a^2b^2 - ab^3 + 3b^4$ by $a + b$.

Step-by-step process:

- (a) **First term of quotient:** Divide the leading term of the dividend by the leading term of the divisor:

$$\frac{3a^4}{a} = 3a^3$$

Multiply $3a^3$ by $(a + b)$: $3a^3(a + b) = 3a^4 + 3a^3b$

Subtract from the dividend:

$$(3a^4 - 5a^3b - 12a^2b^2 - ab^3 + 3b^4) - (3a^4 + 3a^3b) = -8a^3b - 12a^2b^2 - ab^3 + 3b^4$$

- (b) **Second term of quotient:** Divide the new leading term by a :

$$\frac{-8a^3b}{a} = -8a^2b$$

Multiply $-8a^2b$ by $(a + b)$: $-8a^2b(a + b) = -8a^3b - 8a^2b^2$

Subtract:

$$(-8a^3b - 12a^2b^2 - ab^3 + 3b^4) - (-8a^3b - 8a^2b^2) = -4a^2b^2 - ab^3 + 3b^4$$

- (c) **Third term of quotient:** Divide the new leading term by a :

$$\frac{-4a^2b^2}{a} = -4ab^2$$

Multiply $-4ab^2$ by $(a + b)$: $-4ab^2(a + b) = -4a^2b^2 - 4ab^3$

Subtract:

$$(-4a^2b^2 - ab^3 + 3b^4) - (-4a^2b^2 - 4ab^3) = 3ab^3 + 3b^4$$

(d) **Fourth term of quotient:** Divide the new leading term by a :

$$\frac{3ab^3}{a} = 3b^3$$

Multiply $3b^3$ by $(a + b)$: $3b^3(a + b) = 3ab^3 + 3b^4$

Subtract:

$$(3ab^3 + 3b^4) - (3ab^3 + 3b^4) = 0$$

The remainder is zero, confirming that $(a + b)$ divides the product exactly.

Final quotient: $3a^3 - 8a^2b - 4ab^2 + 3b^3$

4. Reduce the following fraction to its lowest terms

$$\frac{x^6 + a^2x^3y}{x^6 - a^4y^2}$$

Solving this problem in no time requires an eagle eye to notice that

$$x^6 - a^4y^2 = (x^3 + a^2y)(x^3 - a^2y)$$

so

$$\frac{x^6 + a^2x^3y}{x^6 - a^4y^2} = \frac{x^3(x^3 + a^2y)}{(x^3 + a^2y)(x^3 - a^2y)} = \frac{x^3}{x^3 - a^2y}$$

5. Simplify

$$\left\{ \frac{a+b}{a-b} + \frac{a-b}{a+b} \right\} \div \left\{ \frac{a+b}{a-b} - \frac{a-b}{a+b} \right\}$$

I find that calculating the numerator and denominator separately is a very straightforward way to answer

$$\frac{a+b}{a-b} + \frac{a-b}{a+b} = \frac{(a+b)^2 + (a-b)^2}{a^2 - b^2} = \frac{a^2 + b^2}{a^2 - b^2}$$

$$\frac{a+b}{a-b} - \frac{a-b}{a+b} = \frac{(a+b)^2 - (a-b)^2}{a^2 - b^2} = \frac{2ab}{a^2 - b^2}$$

Now, division is just multiplying by the reciprocal so:

$$\left\{ \frac{a+b}{a-b} + \frac{a-b}{a+b} \right\} \div \left\{ \frac{a+b}{a-b} - \frac{a-b}{a+b} \right\} = \frac{a^2 + b^2}{a^2 - b^2} \times \frac{a^2 - b^2}{2ab} = \frac{a^2 + b^2}{2ab}$$

6. Solve

$$\frac{3x-4}{2} - \frac{6x-5}{8} = \frac{3x-1}{16}$$

This is an extremely simple exercise, it just takes adding the fractions first

$$\frac{3x-4}{2} - \frac{6x-5}{8} = \frac{8(3x-4) - 2(6x-5)}{16} = \frac{12x-22}{16}$$

the equation is then

$$\frac{12x-22}{16} = \frac{3x-1}{16}$$

or

$$12x-22 = 3x-1$$

which is the same as

$$9x = 21$$

so

$$x = \frac{21}{9} = \frac{7}{3}$$

7. Solve

$$\boxed{7x - 5y = 24, \quad 4x - 3y = 11}$$

We begin by writing the system in the usual forma:

$$7x - 5y = 24$$

$$4x - 3y = 11$$

Now it is easy to see that if we multiply the first eq. by 3 and the second by -5
I we get the equivalent system:

$$21x - 15y = 72$$

$$-20x + 15y = -55$$

adding both equations yield

$$x = 17$$

Substitution of this value in the first equation of the original system,

$$7(17) - 5y = 24,$$

or

$$-5y = 24 - 119 = -95$$

so

$$y = \frac{-95}{-5} = 19$$

The complete solution of the system is thus

$$\boxed{(17, 19)}$$

June 7, 1869